x \in A 
A \cup B = \{x : x \in A or x \in B\}
A \cap B = \{x : x \in A and x \in B\}
A \sub B = \{x \in A : x \not\in B\}

If \{A_i\}_{i\in I} I index set. 
then \big\cup_{i \in I}A_i = {x : x belongs to atleast one A_i}

\big\cap_{i \in I} A_i = {x : x belongs to every A_i}

A \Subset B if x \in A \implies x \in B 

If A is a set, P(A) is the collection of all subsets of A. (power set)

Proposition: $$A \cup B$$ = $$B \cup A$$

$$A \cap B$$ = $$B \cap A$$

A \cup (B \cup C) = (A \cup B) \cup C

A \cap (B \cap C) = (A \cap B) \cap C

A \Subset A \cup B 
A \Subset B iff A \cap B = A

A \cap (B \cup C) = (A cap B) \cup (A \cap C)
A \cup (B\cap C) = (A \cup B) \cap (A \cup C)

A \cup (U_{i\in I} B_i) = U_{i\in I}(A \cap B_i)

A\cup (\cap-{i\in I}B_i) = \cap_{i \in I}(A \cup B_i)

Complements

Suppose X is our universal set.

If A \sub X, A^c = {x \in X : x \in A}

Prop (A \cup B)^c = A^c \cap B^c 
(A \cup  B)^c = A^c \cup B^cap

(\cup_(i \in I) A_i)^c = \cap_{i \in A} A_i^c 

(\cap_(i \in I) A_i)^c = \cup_{i \in A} A_i^c 

Ordered pairs:

A. B are sets:

A \times B = {(a,b) : a \in A, b \in B}

Define (a,b) = {{a}, {a,b}}

$(a,b) = (c,d) \iff a = c and b = d$

Functions:

f : A -> B is a rule that assigns to each a \in A exactly one element f(a) in B

Defn : A function f: A -> B is a subset of \tilde f: A \times B such that for each a \in A \exists ! b \in B s.t. (a,b) \in \tilde f

f : A -> B 
A is the domain
B is the codomain

f(A) = \cup _a \in A {f (a)} = {f(a) : a \in A} is the range or image

f is one to one or injective if f(a) = f(b) => a = b 

f is onto or surjective if for every b \in B \exists a \in A s.t. f(a) = b 

If f : A -> B, S \subset A, f \big\vert_S is the restriction of f to S. 

f \big\vert_S : S -> B, f \big\vert_s = f(s) \forall s \in S 

If T \sub B, then f^(-1) = {a \in A : f(a) \in T} <- inverse image 

f : A -> B, g : B -> C 

g (f (a)) \in C 

g \circ f (a) <- composition

Proposition : f : A -> B 
c, d \in A. E, F \in B
f (c \cup D) = f(c) = f(d)
f(c \cap d) \sub f (c) = f (d) 

f^{-1} (E \cup F) = f^{-1}(E) \cup f^{-1}(F)
f^{-1} (E \cap F) = f^{-1}(E) \cap f^{-1}(F)

(f^{=1}(E))^c = f^{-1} (E^c)

c \sub f^{-1}(f(c))  c \sub A_i
E \cup f(f^-1(E)) E \sub B